deps/poulet4/extraction/Extract.v
@@ -5,36 +5,43 @@ Require Import Coq.extraction.ExtrOcamlNatInt.
 
 Require Import Coq.Numbers.BinNums.
 
-Extract Inductive positive => "Bigint.t"
-  [ "(fun p -> Bigint.of_zarith_bigint (Z.succ (Z.mul (Z.of_int 2) (Bigint.to_zarith_bigint p))))"
-      "(fun p -> Bigint.of_zarith_bigint (Z.mul (Z.of_int 2) (Bigint.to_zarith_bigint p)))" "(Bigint.of_zarith_bigint Z.one)" ]
-  "(fun f2p1 f2p f1 p -> if Z.leq (Bigint.to_zarith_bigint p) Z.one then f1 () else let (q,r) = Z.div_rem (Bigint.to_zarith_bigint p) (Z.of_int 2) in if Z.equal r Z.zero then f2p (Bigint.of_zarith_bigint q) else f2p1 (Bigint.of_zarith_bigint q))".
-
-Extract Inductive Z => "Bigint.t" [ "(Bigint.of_zarith_bigint Z.zero)" "" "(fun z -> Bigint.of_zarith_bigint (Z.neg (Bigint.to_zarith_bigint z)))" ]
-  "(fun fO fp fn z -> let nz = (Bigint.to_zarith_bigint z) in let s = Z.sign nz in if s = 0 then fO () else if s > 0 then fp z else fn (Bigint.of_zarith_bigint (Z.neg nz)))".
-
-Extract Inductive N => "Bigint.t" [ "(Bigint.of_zarith_bigint Z.zero)" "" ]
-  "(fun fO fp n -> if Z.sign (Bigint.to_zarith_bigint n) <= 0 then fO () else fp n)".
-
 Require Poulet4.SimplExpr.
 Require Poulet4.GenLoc.
+Require Poulet4.Syntax.
+Require Poulet4.Typed.
+Require Poulet4.ConstValue.
+Require Poulet4.P4cub.GCL.
+Require Poulet4.ToP4cub.
+Require Poulet4.P4cub.ToGCL.
+
+
+Extract Inductive positive => "Bigint.t"
+  [ "(fun p -> Bigint.of_zarith_bigint (Z.succ (Z.mul (Z.of_int 2) (Bigint.to_zarith_bigint p))))"
+      "(fun p -> Bigint.of_zarith_bigint (Z.mul (Z.of_nat 2) (Bigint.to_zarith_bigint p)))" "(Bigint.of_zarith_bigint (Z.of_nat 1))" ]
+  "(fun f2p1 f2p f1 p -> if Z.leq (Bigint.to_zarith_bigint p) (Z.of_nat 1) then f1 () else let (q,r) = Z.div_rem (Bigint.to_zarith_bigint p) (Z.of_int 2) in if Z.equal r (Z.of_nat 0) then f2p (Bigint.of_zarith_bigint q) else f2p1 (Bigint.of_zarith_bigint q))".
+
+Extract Inductive Z => "Bigint.t" [ "(Bigint.of_zarith_bigint (Z.of_nat 0))" "" "(fun z -> Bigint.of_zarith_bigint (Z.neg (Bigint.to_zarith_bigint z)))" ]
+  "(fun fO fp fn z -> let nz = (Bigint.to_zarith_bigint z) in let s = Z.sign nz in if s = 0 then fO () else if s > 0 then fp z else fn (Bigint.of_zarith_bigint (Z.neg nz)))".
+
+Extract Inductive N => "Bigint.t" [ "(Bigint.of_zarith_bigint (Z.of_nat 0))" "" ]
+  "(fun fO fp n -> if Z.sign (Bigint.to_zarith_bigint n) <= 0 then fO () else fp n)".
+
 
 Extract Constant SyntaxUtil.dummy_ident => "(fun () -> failwith ""unrealized dummy_ident reached"")".
 Extract Constant SimplExpr.to_digit => "(fun x -> Char.chr 20)".
 Extract Constant SimplExpr.N_to_string_aux => "(fun x y z -> z)". (* Don't remove: this line informs Coq to not actually extract this function. *)
 Extract Constant SimplExpr.N_to_string => "(fun x -> Z.to_string (Bigint.to_zarith_bigint x))".
 Extract Constant SimplExpr.add1 => "(fun x -> Bigint.of_zarith_bigint (Z.succ (Bigint.to_zarith_bigint x)))".
-Extract Inlined Constant SimplExpr.Nzero => "(Bigint.of_zarith_bigint Z.zero)".
+Extract Inlined Constant SimplExpr.Nzero => "(Bigint.of_zarith_bigint (Z.of_int 0))".
 Extract Inlined Constant BinNat.N.eqb => "Bigint.(=)".
 Extract Inlined Constant BinNat.N.add => "Bigint.(+)".
 Extract Inlined Constant Nat.add => "(+)".
-
-Require Poulet4.Syntax.
-Require Poulet4.Typed.
-Require Poulet4.ConstValue.
 
 
 Separate Extraction Poulet4.Syntax
          Poulet4.Typed Poulet4.SimplExpr
          Poulet4.GenLoc
-         Poulet4.ConstValue.
+         Poulet4.ConstValue
+         Poulet4.ToP4cub
+         Poulet4.P4cub.GCL
+         Poulet4.P4cub.ToGCL.
