deps/poulet4/lib/P4cub/Architecture/Architecture.v
@@ -2,6 +2,7 @@ Set Warnings "-custom-entry-overridden".
 Require Import Poulet4.P4cub.Syntax.AST
         Poulet4.P4cub.Architecture.Paquet
         Poulet4.P4cub.Envn.
+Import String.
 
 (** P4cub's analogue to p4light's [Target.v].
     May be replace entirely with [Target.v]
