deps/poulet4/lib/P4cub/BigStep/IndPrincip.v
@@ -4,6 +4,7 @@ Require Import Poulet4.P4cub.Envn
         Poulet4.P4cub.BigStep.Value.Value
         Poulet4.P4cub.BigStep.Semantics
         Coq.ZArith.BinInt.
+Import String.
 Import Step AllCubNotations Val.ValueNotations.
 
 (** A custom induction principle for
