deps/poulet4/lib/P4cub/Static/Typing.v
@@ -3,7 +3,7 @@ Require Import Coq.PArith.BinPos Coq.ZArith.BinInt Coq.NArith.BinNat
         Poulet4.P4cub.Syntax.AST Poulet4.P4Arith
         Poulet4.P4cub.Envn Poulet4.P4cub.Static.Util
         Poulet4.P4cub.Syntax.CubNotations.
-
+Import String.
 (* TODO: type parameters, arguments, ok types. *)
 
 (** Expression typing. *)
